refactor(Modal): Refactor Hilbert Systems (#451)

Foundation/Modal/Logic/Dz/Basic.lean
@@ -6,76 +6,76 @@ namespace LO.Modal
 open Formula (atom)
 open Logic
 
-protected abbrev Logic.Dz := sumQuasiNormal Logic.GL {∼□⊥, □(□(.atom 0) ⋎ □(.atom 1)) ➝ □(.atom 0) ⋎ □(.atom 1)}
-instance : Logic.Dz.IsQuasiNormal := inferInstance
+protected abbrev Dz := sumQuasiNormal Modal.GL {∼□⊥, □(□(.atom 0) ⋎ □(.atom 1)) ➝ □(.atom 0) ⋎ □(.atom 1)}
+instance : Modal.Dz.IsQuasiNormal := inferInstance
 
-instance : Entailment.HasAxiomP Logic.Dz where
+instance : Entailment.HasAxiomP Modal.Dz where
   P := by
     constructor;
     apply Logic.sumQuasiNormal.mem₂;
     simp;
 
-lemma Logic.Dz.mem_axiomDz : Logic.Dz ⊢! □(□φ ⋎ □ψ) ➝ □φ ⋎ □ψ := by
+lemma Dz.mem_axiomDz : Modal.Dz ⊢! □(□φ ⋎ □ψ) ➝ □φ ⋎ □ψ := by
   apply Logic.subst! (φ := □(□(.atom 0) ⋎ □(.atom 1)) ➝ □(.atom 0) ⋎ □(.atom 1)) (s := λ a => if a = 0 then φ else ψ);
   apply Logic.sumQuasiNormal.mem₂!;
   simp;
 
-instance : Logic.GL ⪱ Logic.Dz := by
+instance : Modal.GL ⪱ Modal.Dz := by
   constructor;
   . infer_instance;
   . apply Entailment.not_weakerThan_iff.mpr;
     use ∼□⊥;
     constructor;
     . simp;
-    . exact Logic.GL.unprovable_notbox;
+    . simpa using GL.unprovable_notbox;
 
 section
 
-private inductive Logic.Dz.aux : Logic ℕ
-  | mem_GL {φ} : Logic.GL ⊢! φ → Logic.Dz.aux φ
-  | axiomP : Logic.Dz.aux (∼□⊥)
-  | axiomDz (φ ψ) : Logic.Dz.aux (□(□φ ⋎ □ψ) ➝ □φ ⋎ □ψ)
-  | mdp  {φ ψ} : Logic.Dz.aux (φ ➝ ψ) → Logic.Dz.aux φ → Logic.Dz.aux ψ
+private inductive Dz' : Logic ℕ
+  | mem_GL {φ} : Modal.GL ⊢! φ → Modal.Dz' φ
+  | axiomP : Modal.Dz' (∼□⊥)
+  | axiomDz (φ ψ) : Modal.Dz' (□(□φ ⋎ □ψ) ➝ □φ ⋎ □ψ)
+  | mdp  {φ ψ} : Modal.Dz' (φ ➝ ψ) → Modal.Dz' φ → Modal.Dz' ψ
 
-private lemma Logic.Dz.eq_aux : Logic.Dz = Logic.Dz.aux := by
+private lemma Dz'.eq_Dz : Modal.Dz' = Modal.Dz := by
   ext φ;
   constructor;
-  . intro h;
-    induction h with
-    | mem₁ h => exact Logic.Dz.aux.mem_GL h;
-    | mem₂ h =>
-      rcases h with (rfl | rfl);
-      . apply Logic.Dz.aux.axiomP;
-      . apply Logic.Dz.aux.axiomDz;
-    | mdp _ _ ihφψ ihφ => exact Logic.Dz.aux.mdp ihφψ ihφ;
-    | subst hφ ihφ =>
-      clear hφ;
-      induction ihφ with
-      | mem_GL h =>
-        apply Logic.Dz.aux.mem_GL;
-        apply subst!;
-        exact h;
-      | axiomP => apply Logic.Dz.aux.axiomP;
-      | axiomDz _ _ => apply Logic.Dz.aux.axiomDz;
-      | mdp _ _ ihφψ ihφ => apply Logic.Dz.aux.mdp ihφψ ihφ;
   . intro h;
     apply iff_provable.mp;
     induction h with
     | mem_GL h => exact sumQuasiNormal.mem₁! h;
     | mdp _ _ ihφψ ihφ => exact ihφψ ⨀ ihφ;
-    | axiomDz φ => apply Logic.Dz.mem_axiomDz;
+    | axiomDz φ => apply Modal.Dz.mem_axiomDz;
     | axiomP => simp;
+  . intro h;
+    induction h with
+    | mem₁ h => exact Modal.Dz'.mem_GL h;
+    | mem₂ h =>
+      rcases h with (rfl | rfl);
+      . apply Modal.Dz'.axiomP;
+      . apply Modal.Dz'.axiomDz;
+    | mdp _ _ ihφψ ihφ => exact Modal.Dz'.mdp ihφψ ihφ;
+    | subst hφ ihφ =>
+      clear hφ;
+      induction ihφ with
+      | mem_GL h =>
+        apply Modal.Dz'.mem_GL;
+        apply subst!;
+        exact h;
+      | axiomP => apply Modal.Dz'.axiomP;
+      | axiomDz _ _ => apply Modal.Dz'.axiomDz;
+      | mdp _ _ ihφψ ihφ => apply Modal.Dz'.mdp ihφψ ihφ;
 
 -- TODO: Remove `eq_Dz_Dz'`?
-protected def Logic.Dz.rec'
-  {motive : (φ : Formula ℕ) → (Logic.Dz ⊢! φ) → Prop}
-  (mem_GL : ∀ {φ}, (h : Logic.GL ⊢! φ) → motive φ (sumQuasiNormal.mem₁! h))
+protected def Dz.rec'
+  {motive : (φ : Formula ℕ) → (Modal.Dz ⊢! φ) → Prop}
+  (mem_GL : ∀ {φ}, (h : Modal.GL ⊢! φ) → motive φ (sumQuasiNormal.mem₁! h))
   (axiomP : motive (∼□⊥) (by simp))
-  (axiomDz : ∀ {φ ψ}, motive (□(□φ ⋎ □ψ) ➝ □φ ⋎ □ψ) (Logic.Dz.mem_axiomDz))
-  (mdp : ∀ {φ ψ}, {hφψ : Logic.Dz ⊢! φ ➝ ψ} → {hφ : Logic.Dz ⊢! φ} → (motive (φ ➝ ψ) hφψ) → (motive φ hφ) → motive ψ (hφψ ⨀ hφ))
-  : ∀ {φ}, (h : Logic.Dz ⊢! φ) → motive φ h := by
+  (axiomDz : ∀ {φ ψ}, motive (□(□φ ⋎ □ψ) ➝ □φ ⋎ □ψ) (Modal.Dz.mem_axiomDz))
+  (mdp : ∀ {φ ψ}, {hφψ : Modal.Dz ⊢! φ ➝ ψ} → {hφ : Modal.Dz ⊢! φ} → (motive (φ ➝ ψ) hφψ) → (motive φ hφ) → motive ψ (hφψ ⨀ hφ))
+  : ∀ {φ}, (h : Modal.Dz ⊢! φ) → motive φ h := by
   intro φ h;
-  replace h := iff_provable.mp $ Logic.Dz.eq_aux.symm ▸ h;
+  replace h := iff_provable.mp $ Modal.Dz'.eq_Dz ▸ h;
   induction h with
   | mem_GL h => apply mem_GL; assumption;
   | axiomP => apply axiomP;
@@ -85,9 +85,9 @@ protected def Logic.Dz.rec'
     . apply ihφψ;
     . apply ihφ;
     . replace hφψ := iff_provable.mpr hφψ;
-      rwa [←Logic.Dz.eq_aux] at hφψ;
+      rwa [Dz'.eq_Dz] at hφψ;
     . replace hφ := iff_provable.mpr hφ;
-      rwa [←Logic.Dz.eq_aux] at hφ;
+      rwa [Dz'.eq_Dz] at hφ;
 
 end
 
