Foundation.lean
@@ -81,11 +81,8 @@ import Foundation.IntFO.Translation
 -- import Foundation.Propositional.Dialectica.Basic
 
 -- Modal
-import Foundation.Modal.Hilbert.KP
-import Foundation.Modal.Hilbert.S5Grz
-import Foundation.Modal.Hilbert.GL.Alternatives
-import Foundation.Modal.Hilbert.Minimal.Basic
 import Foundation.Modal.Hilbert.K_EMCN
+import Foundation.Modal.Hilbert.GL_K4Loeb_K4Henkin_K4Hen
 
 import Foundation.Modal.Kripke.Logic.GL.Unnecessitation
 import Foundation.Modal.Kripke.Logic.GL.MDP
