Foundation/Modal/Kripke/Logic/K4.lean
@@ -1,4 +1,4 @@
-import Foundation.Modal.Hilbert.WellKnown
+import Foundation.Modal.Hilbert.Normal.Basic
 import Foundation.Modal.Kripke.AxiomGeach
 import Foundation.Modal.Kripke.Hilbert
 import Foundation.Modal.Kripke.Filtration
@@ -11,6 +11,7 @@ open Formula
 open Kripke
 open Hilbert.Kripke
 
+
 namespace Kripke
 
 abbrev Frame.IsK4 (F : Frame) := F.IsTransitive
@@ -22,30 +23,32 @@ protected abbrev FrameClass.finite_K4 : FrameClass := { F | F.IsFiniteK4 }
 end Kripke
 
 
-namespace Logic.K4.Kripke
+namespace Hilbert
 
-instance sound : Sound Logic.K4 FrameClass.K4 := instSound_of_validates_axioms $ by
+namespace K4.Kripke
+
+instance : Sound Hilbert.K4 FrameClass.K4 := instSound_of_validates_axioms $ by
   apply FrameClass.Validates.withAxiomK;
   rintro F F_trans φ rfl;
   apply validate_AxiomFour_of_transitive (trans := F_trans);
 
-instance consistent : Entailment.Consistent Logic.K4 :=
+instance : Entailment.Consistent Hilbert.K4 :=
   consistent_of_sound_frameclass FrameClass.K4 $ by
     use whitepoint;
     apply Set.mem_setOf_eq.mpr;
     infer_instance;
 
-instance canonical : Canonical Logic.K4 FrameClass.K4 := ⟨by
+instance : Canonical Hilbert.K4 FrameClass.K4 := ⟨by
   apply Set.mem_setOf_eq.mpr;
   infer_instance;
 ⟩
 
-instance complete : Complete Logic.K4 FrameClass.K4 := inferInstance
+instance : Complete Hilbert.K4 FrameClass.K4 := inferInstance
 
 open finestFiltrationTransitiveClosureModel in
-instance finite_complete : Complete Logic.K4 FrameClass.finite_K4 := ⟨by
+instance : Complete Hilbert.K4 FrameClass.finite_K4 := ⟨by
   intro φ hp;
-  apply Kripke.complete.complete;
+  apply Complete.complete (𝓜 := FrameClass.K4);
   intro F F_trans V x;
   replace F_trans := Set.mem_setOf_eq.mp F_trans;
   let M : Kripke.Model := ⟨F, V⟩;
@@ -56,17 +59,17 @@ instance finite_complete : Complete Logic.K4 FrameClass.finite_K4 := ⟨by
   exact { world_finite := by apply FilterEqvQuotient.finite $ by simp }
 ⟩
 
-lemma trans : Logic.K4 = FrameClass.K4.logic := eq_hilbert_logic_frameClass_logic
+end K4.Kripke
 
-instance : Logic.K ⪱ Logic.K4 := by
+instance : Hilbert.K ⪱ Hilbert.K4 := by
   constructor;
-  . apply Hilbert.weakerThan_of_subset_axioms $ by simp;
+  . apply Hilbert.Normal.weakerThan_of_subset_axioms $ by simp;
   . apply Entailment.not_weakerThan_iff.mpr;
-    suffices ∃ φ, Logic.K4 ⊢! φ ∧ ¬FrameClass.all ⊧ φ by simpa [K.Kripke.all];
     use (Axioms.Four (.atom 0));
     constructor;
     . simp;
-    . apply Kripke.not_validOnFrameClass_of_exists_model_world;
+    . apply Sound.not_provable_of_countermodel (𝓜 := FrameClass.all)
+      apply Kripke.not_validOnFrameClass_of_exists_model_world;
       let M : Model := ⟨⟨Fin 2, λ x y => x ≠ y⟩, λ w _ => w = 1⟩;
       use M, 0;
       constructor
@@ -80,6 +83,9 @@ instance : Logic.K ⪱ Logic.K4 := by
           | 1 => tauto;
         . exact ⟨1, by omega, 0, by omega, by trivial⟩;
 
-end Logic.K4.Kripke
+end Hilbert
+
+instance : Modal.K ⪱ Modal.K4 := inferInstance
+
 
 end LO.Modal
