Foundation/Modal/Kripke/Logic/K5.lean
@@ -1,6 +1,6 @@
 import Foundation.Modal.Kripke.AxiomGeach
 import Foundation.Modal.Kripke.Hilbert
-import Foundation.Modal.Hilbert.WellKnown
+import Foundation.Modal.Hilbert.Normal.Basic
 import Foundation.Modal.Kripke.Logic.K
 
 namespace LO.Modal
@@ -19,38 +19,39 @@ abbrev FrameClass.K5 : FrameClass := { F | F.IsK5 }
 end Kripke
 
 
-namespace Logic.K5.Kripke
+namespace Hilbert
 
-instance sound : Sound (Logic.K5) Kripke.FrameClass.K5 := instSound_of_validates_axioms $ by
+namespace K5.Kripke
+
+instance : Sound Hilbert.K5 FrameClass.K5 := instSound_of_validates_axioms $ by
   apply FrameClass.Validates.withAxiomK;
   rintro F F_eucl _ rfl;
   exact validate_AxiomFive_of_euclidean (eucl := F_eucl);
 
-instance consistent : Entailment.Consistent (Logic.K5) :=
-  consistent_of_sound_frameclass Kripke.FrameClass.K5 $ by
+instance : Entailment.Consistent Hilbert.K5 :=
+  consistent_of_sound_frameclass FrameClass.K5 $ by
     use whitepoint;
     apply Set.mem_setOf_eq.mpr;
     infer_instance;
 
-instance canonical : Canonical (Logic.K5) Kripke.FrameClass.K5 := ⟨by
+instance : Canonical Hilbert.K5 FrameClass.K5 := ⟨by
   apply Set.mem_setOf_eq.mpr;
   infer_instance;
 ⟩
 
-instance complete : Complete (Logic.K5) Kripke.FrameClass.K5 := inferInstance
+instance : Complete Hilbert.K5 FrameClass.K5 := inferInstance
 
-lemma eucl : Logic.K5 = Kripke.FrameClass.K5.logic := eq_hilbert_logic_frameClass_logic
+end K5.Kripke
 
-instance : Logic.K ⪱ Logic.K5 := by
+instance : Hilbert.K ⪱ Hilbert.K5 := by
   constructor;
-  . apply Hilbert.weakerThan_of_subset_axioms $ by simp;
+  . apply Hilbert.Normal.weakerThan_of_subset_axioms $ by simp;
   . apply Entailment.not_weakerThan_iff.mpr;
-    suffices ∃ φ, Logic.K5 ⊢! φ ∧ ¬FrameClass.all ⊧ φ by
-      simpa [K.Kripke.all];
     use (Axioms.Five (.atom 0));
     constructor;
-    . exact axiomFive!;
-    . apply Kripke.not_validOnFrameClass_of_exists_model_world;
+    . simp;
+    . apply Sound.not_provable_of_countermodel (𝓜 := FrameClass.all)
+      apply Kripke.not_validOnFrameClass_of_exists_model_world;
       let M : Model := ⟨⟨Fin 2, λ x _ => x = 0⟩, λ w _ => w = 0⟩;
       use M, 0;
       constructor;
@@ -59,6 +60,9 @@ instance : Logic.K ⪱ Logic.K5 := by
         use 1;
         trivial;
 
-end Logic.K5.Kripke
+end Hilbert
+
+instance : Modal.K ⪱ Modal.K5 := inferInstance
+
 
 end LO.Modal
