Foundation/Modal/Kripke/Logic/KD4Point3Z.lean
@@ -1,6 +1,6 @@
 import Foundation.Modal.Kripke.AxiomL
 import Foundation.Modal.Kripke.Logic.Soundness
-import Foundation.Modal.Hilbert.WellKnown
+import Foundation.Modal.Hilbert.Normal.Basic
 import Foundation.Modal.Kripke.LinearFrame
 import Foundation.Modal.Kripke.AxiomWeakPoint3
 import Foundation.Modal.Kripke.AxiomGeach
@@ -16,7 +16,7 @@ open Hilbert.Kripke
 
 namespace Logic.KD4Point3Z.Kripke
 
-instance sound_natLT : Sound Hilbert.KD4Point3Z natLT := instSound_of_frame_validates_axioms $ by
+instance : Sound Hilbert.KD4Point3Z natLT := instSound_of_frame_validates_axioms $ by
   simp only [Semantics.RealizeSet.insert_iff, ValidOnFrame.models_iff, Semantics.RealizeSet.singleton_iff];
   refine ⟨?_, ?_, ?_, ?_, ?_⟩;
   . apply FrameClass.all.validates_axiomK <;> tauto;
@@ -25,7 +25,7 @@ instance sound_natLT : Sound Hilbert.KD4Point3Z natLT := instSound_of_frame_vali
   . apply validate_WeakPoint3_of_weakConnected;
   . apply Kripke.natLT_validates_AxiomZ;
 
-instance consistent : Entailment.Consistent Logic.KD4Point3Z := consistent_of_sound_frames natLT
+instance : Entailment.Consistent Logic.KD4Point3Z := consistent_of_sound_frames natLT
 
 end Logic.KD4Point3Z.Kripke
 
